Cleanup the uint model a bit

src/Helpers/MachinePrimitives.v
@@ -11,40 +11,43 @@ Instance eqdecision `{dec:EqualDec A} : EqDecision A := dec.
 From Coq Require Import NArith.NArith.
 Local Open Scope N.
 
-Axiom ByteString : Type.
-Axiom eqdec_ByteString : EqualDec ByteString.
-Existing Instance eqdec_ByteString.
+(** Machine unsigned integers *)
 
-Record MachineUint (bits:nat) : Type :=
+Record MachineUInt (bytes:nat) : Type :=
   { intTy :> Type;
     intPlus : intTy -> intTy -> intTy;
     intSub : intTy -> intTy -> intTy;
     intCmp : intTy -> intTy -> comparison;
     fromNum : N -> intTy;
+    int_val0 := fromNum 0;
+    int_val1 := fromNum 1;
     toNum : intTy -> N;
     toNum_inj : forall x y, toNum x = toNum y -> x = y;
     intCmp_ok : forall x y, intCmp x y = N.compare (toNum x) (toNum y);
-    toNum_ok : forall x, toNum x < N.pow 2 (N.of_nat bits);
-    encodeLE : intTy -> ByteString;
-    decodeLE : ByteString -> intTy;
-    encode_decode_LE_ok : forall x, decodeLE (encodeLE x) = x; }.
+    toNum_ok : forall x, toNum x < N.pow 2 (8 * N.of_nat bytes);
+  }.
 
-Definition int_val0 bits {int:MachineUint bits} := int.(fromNum) 0.
-Definition int_val1 bits {int:MachineUint bits} := int.(fromNum) 1.
-Arguments intCmp {bits int} : rename.
-Arguments intSub {bits int} : rename.
-Arguments toNum {bits int} : rename.
+Arguments int_val0 {bytes int} : rename.
+Arguments int_val1 {bytes int} : rename.
+Arguments intCmp {bytes int} : rename.
+Arguments intSub {bytes int} : rename.
+Arguments toNum {bytes int} : rename.
 
-Instance uint_eqdec bits (int: MachineUint bits) : EqualDec int.
+Instance uint_eqdec bytes (int: MachineUInt bytes) : EqualDec int.
 Proof.
-  apply (EqualDec.inj_eq_dec toNum).
-  apply toNum_inj.
+  hnf; intros.
+  destruct_with_eqn (intCmp x y);
+    [ left | right; intros -> .. ];
+    rewrite intCmp_ok, ?N.compare_eq_iff, ?N.compare_refl in *.
+  - auto using toNum_inj.
+  - congruence.
+  - congruence.
 Defined.
 
-Axiom uint64 : MachineUint 64.
-Axiom uint32 : MachineUint 32.
-Axiom uint16 : MachineUint 16.
-Axiom uint8   : MachineUint 8.
+Axiom uint64 : MachineUInt 8.
+Axiom uint32 : MachineUInt 4.
+Axiom uint16 : MachineUInt 2.
+Axiom uint8  : MachineUInt 1.
 
 Definition uint_val4096 : uint64 := uint64.(fromNum) 4096.
 
@@ -52,6 +55,10 @@ Axiom uint64_to_uint16 : uint64 -> uint16.
 Axiom uint64_to_uint32 : uint64 -> uint32.
 Axiom uint16_to_uint64 : uint16 -> uint64.
 Axiom uint32_to_uint64 : uint32 -> uint64.
+
+Axiom ByteString : Type.
+Axiom eqdec_ByteString : EqualDec ByteString.
+Existing Instance eqdec_ByteString.
 
 Module BS.
   Axiom append : ByteString -> ByteString -> ByteString.
@@ -69,6 +76,21 @@ Module BSNotations.
   Delimit Scope bs_scope with bs.
   Infix "++" := BS.append : bs_scope.
 End BSNotations.
+
+Class UIntEncoding bytes (int: MachineUInt bytes) : Type :=
+  { encodeLE : int -> ByteString;
+    decodeLE : ByteString -> option int;
+    encode_length_ok : forall x, toNum (BS.length (encodeLE x)) = N.of_nat bytes;
+    encode_decode_LE_ok : forall x, decodeLE (encodeLE x) = Some x;
+  }.
+
+Axiom uint64_le_enc : UIntEncoding uint64.
+Axiom uint32_le_enc : UIntEncoding uint32.
+Axiom uint16_le_enc : UIntEncoding uint16.
+Axiom uint8_le_enc : UIntEncoding uint8.
+Existing Instances uint64_le_enc uint32_le_enc uint16_le_enc uint8_le_enc.
+
+(** File descriptors *)
 
 Axiom Fd:Type.
 Axiom fd_eqdec : EqualDec Fd.
